When taking $n$ success/failure trials and $P[1]=p$, the probability of $n_0$ 0's and $n_1$ 1's is  
$P[E_{n_0,n_1}]=\dbinom{n}{n_1}(1-p)^{n-n_1}p^{n_1}=\dbinom{n}{n_0}(1-p)^{n_0}p^{n-n_0}$ 
## what idk figure this out later (i never did)
theorem 2.9 ch 2 slide 50  
When taking $n=n_0+\cdots+n_{m-1}$ independent trials from sample space $S=\{s_0,\cdots,s_{m-1}\}$ with $P[s_i]=p_i$, the probability of $n_i$ occurences of $s_i$, $i=0,1,\dotsm-1$ is  
$P[E_{n0},\dots,n_{m-1}]=\binom{n}{n_0,\dots,n_{m-1}}p_0^{n_0}\dots p_{m-1}^{m-1}$

___

< [[Spring 2024/EEC161/Notes/Counting Methods|Counting Methods]] | Current Page | [[Spring 2024/EEC161/Notes/Reliability Analysis|Reliability Analysis]] >